feat: enhance handling of `undef` and `freeze` instructions in semantics, add corresponding tests

LeanNanoLlvm/Semantics/State.lean
@@ -20,6 +20,7 @@ instance : ToString RegisterValue where
 
 structure NanoLlvmState : Type where
   (registers : ExtHashMap AST.Identifier RegisterValue)
+  (undefs : ExtHashMap AST.RawId RegisterValue)
   -- TODO: memory
   -- (memory : ExtHashMap MemoryAddress MemoryValue)
 
